theories/goedel/PRrepresentable.v
@@ -521,7 +521,7 @@ Proof.
                      repeat
                       (rewrite (subTermNil LNN (natToTerm a)); [| apply closedNatToTerm ]).
                      replace
-                      (fol.equal 
+                      (equal 
                          (apply LNN Languages.Plus
                             (Tcons
                                (apply LNN Languages.Times
@@ -889,7 +889,7 @@ Proof.
         repeat rewrite (subFormulaEqual LNN). simpl in |- *.
         destruct (Nat.eq_dec n n); try lia.
         replace
-          (fol.equal  (var 0)
+          (equal  (var 0)
             (substituteTerm LNN (natToTerm a) (S n)
               (natToTerm a0)))
           with
@@ -1023,7 +1023,7 @@ Proof.
            iffTrans
              with
               (existH (n + S w)
-                 (andH (fol.equal (var (S (n + w))) (natToTerm (snd a)))
+                 (andH (equal (var (S (n + w))) (natToTerm (snd a)))
                     (addExists (S w) n
                        (andH (FormulasToFormula 0 w n v)
                           (subAllFormula LNN B
@@ -1040,17 +1040,17 @@ Proof.
                     (SysPrf
                        (Ensembles.Add (fol.Formula LNN) NN
                           (andH
-                             (andH (fol.equal  (var (S (n + w))) (natToTerm (snd a)))
+                             (andH (equal  (var (S (n + w))) (natToTerm (snd a)))
                                 (FormulasToFormula 0 w n v))
                              (subAllFormula LNN B
                                 (fun x : nat =>
                                  match x with
                                  | O => var 0
                                  | S x' => var (S (x' + w))
-                                 end)))) (fol.equal (var (S (n + w))) (natToTerm (snd a)))).
+                                 end)))) (equal (var (S (n + w))) (natToTerm (snd a)))).
                    +++ generalize
                         (andH
-                           (andH (fol.equal (var (S (n + w))) (natToTerm (snd a)))
+                           (andH (equal (var (S (n + w))) (natToTerm (snd a)))
                               (FormulasToFormula 0 w n v))
                            (subAllFormula LNN B
                               (fun x : nat =>
@@ -1076,7 +1076,7 @@ Proof.
                          with
                            (addExists (S w) n
                               (andH
-                                 (andH (fol.equal (var (S (n + w))) (natToTerm (snd a)))
+                                 (andH (equal (var (S (n + w))) (natToTerm (snd a)))
                                     (FormulasToFormula 0 w n v))
                                  (subAllFormula LNN B
                                     (fun x : nat =>
@@ -1104,12 +1104,12 @@ Proof.
                                  | O => var 0
                                  | S x' => var (S (x' + w))
                                  end)))).
-                   +++ apply impE with (fol.equal (var (S (n + w))) (natToTerm (snd a))).
+                   +++ apply impE with (equal (var (S (n + w))) (natToTerm (snd a))).
                        --- apply sysWeaken. apply impI.
                            cut
                             (SysPrf
                                (Ensembles.Add (fol.Formula LNN) NN
-                                  (fol.equal (var (S (n + w))) (natToTerm (snd a))))
+                                  (equal (var (S (n + w))) (natToTerm (snd a))))
                                (impH
                                   (andH (FormulasToFormula 0 w n v)
                                      (subAllFormula LNN B
@@ -1119,7 +1119,7 @@ Proof.
                                          | S x' => var (S (x' + w))
                                          end)))
                                   (andH
-                                     (andH (fol.equal (var (S (n + w))) (natToTerm (snd a)))
+                                     (andH (equal (var (S (n + w))) (natToTerm (snd a)))
                                         (FormulasToFormula 0 w n v))
                                      (subAllFormula LNN B
                                         (fun x : nat =>
@@ -1136,7 +1136,7 @@ Proof.
                                        | S x' => var (S (x' + w))
                                        end)))
                                 (andH
-                                   (andH (fol.equal (var (S (n + w))) (natToTerm (snd a)))
+                                   (andH (equal (var (S (n + w))) (natToTerm (snd a)))
                                       (FormulasToFormula 0 w n v))
                                    (subAllFormula LNN B
                                       (fun x : nat =>
@@ -1406,684 +1406,15 @@ Proof.
   + apply H; auto.
 Qed.
 
-(*
-Local composePiFormula [n,w,m:nat][A:(vector Formula*(naryFunc n) m)][B:Formula] : Formula :=
-(addForalls (S w) m (impH (FormulasToFormula n w m A)
-(subAllFormula LNN B [x:nat]
-     (Cases x of O => (var O) | (S x')=>(var (plus (S x') w))end)))).
 
-Remark composePiRepresentable : (n,w,m:nat)(le n w)->(A:(vector Formula*(naryFunc n) m))
-(B:Formula)(g:(naryFunc m))
-(RepresentablesHelp n m A)->
-(vector_rect Formula*(naryFunc n) [_][_]Prop
- True
- [pair:(Formula*(naryFunc n))][m:nat][v:(vector ? m)][rec:Prop]
- ((v:nat)(In v (freeVarFormula LNN (Fst pair)))->(le v n))/\rec
-  m A)->
-(Representable m g B)->
-(Representable n (evalComposeFunc n m (FormulasToFuncs n m A) g)
- (composePiFormula n w m A B)).
-Proof.
-Assert (n,w,m:nat)(le n w)->(A:(vector Formula*(naryFunc n) m))
-(B:Formula)(g:(naryFunc m))
-(RepresentablesHelp n m A)->
-(vector_rect Formula*(naryFunc n) [_][_]Prop
- True
- [pair:(Formula*(naryFunc n))][m:nat][v:(vector ? m)][rec:Prop]
- ((v:nat)(In v (freeVarFormula LNN (Fst pair)))->(le v n))/\rec
-  m A)->
-(Representable m g B)->
-(RepresentableHelp n (evalComposeFunc n m (FormulasToFuncs n m A) g)
- (composePiFormula n w m A B)).
-Intro.
-Induction n; Simpl.
-Intros w m H v.
-Induction v; Simpl; Intros.
-Unfold composePiFormula.
-Simpl.
-Replace (subAllFormula LNN B
-           [x:nat]
-            Cases x of
-              0 => (var (0))
-            | (S x') => (var (S (plus x' w)))
-            end)
-with (subAllFormula LNN B [x:nat](var x)).
-Apply iffTrans with B.
-Apply iffTrans with (subAllFormula LNN B [x:nat](var x)).
-Apply iffI;
-Apply impI.
-Apply impE with (equal (var (0)) (var (0))).
-Apply Axm; Right; Constructor.
-Apply eqRefl.
-Apply impI.
-Apply Axm; Left; Right; Constructor.
-Apply (subAllFormulaId LNN).
-Induction H2.
-Auto.
-Apply subAllFormula_ext.
-Intros.
-NewDestruct m.
-Auto.
-Elim (le_Sn_O n).
-Induction H2.
-Apply H2.
-Auto.
-Induction H0.
-Induction H1.
-Induction H2.
-Assert (a:nat)(SysPrf NN
-	    (iffH (composePiFormula (0) w n v (substituteFormula LNN B (S n) (natToTerm a)))
-              (equal (var (0))
-                (natToTerm
-                  (evalList n (FormulasToFuncs (0) n v) (g a)))))).
-Intros.
-Apply Hrecv.
-Auto.
-Auto.
-Split.
-Intros.
-NewInduction (freeVarSubFormula3 ? ? ? ? ? H6).
-Assert (In v0 (freeVarFormula LNN B)).
-EApply In_list_remove1.
-Apply H7.
-NewInduction (le_lt_or_eq ? ? (H2 ? H8)).
-Apply lt_n_Sm_le.
-Auto.
-Elim (In_list_remove2 ? ? ? ? ? H7).
-Auto.
-Elim (closedNatToTerm ? ? H7).
-Apply H5.
-Clear Hrecv.
-Unfold composePiFormula.
-Unfold composePiFormula in H6.
-Simpl.
-Apply iffTrans with (addForalls (S w) n
-              (impH (FormulasToFormula (0) w n v)
-                (subAllFormula LNN
-                  (substituteFormula LNN B (S n) (natToTerm (Snd a)))
-                  [x:nat]
-                   Cases x of
-                     0 => (var (0))
-                   | (S x') => (var (S (plus x' w)))
-                   end)));
-[Idtac | Apply H6].
-Clear H6.
-Apply iffTrans with (forallH (plus n (S w))
-         (addForalls (S w) n
-           (impH
-             (andH
-               (substituteFormula LNN (equal (var (0)) (natToTerm (Snd a))) (0) (var (S (plus n w))))
-               (FormulasToFormula (0) w n v))
-             (subAllFormula LNN B
-               [x:nat]
-                Cases x of
-                  0 => (var (0))
-                | (S x') => (var (S (plus x' w)))
-                end)))).
-Apply (reduceForall LNN).
-Apply closedNN.
-Apply reduceAddForalls.
-Apply (reduceImp LNN); Try Apply iffRefl.
-Apply (reduceAnd LNN); Try Apply iffRefl.
-Apply (reduceSub LNN).
-Apply closedNN.
-Auto.
-Rewrite (subFormulaEqual LNN).
-Rewrite (subTermVar1 LNN).
-Rewrite (subTermNil LNN).
-Apply iffTrans with (forallH (plus n (S w))
-       (impH         (fol.equal LNN (var (S (plus n w))) (natToTerm (Snd a)))
-        (addForalls (S w) n
-             (impH
-               (FormulasToFormula (0) w n v)
-             (subAllFormula LNN B
-               [x:nat]
-                Cases x of
-                  0 => (var (0))
-                | (S x') => (var (S (plus x' w)))
-                end))))).
-Apply (reduceForall LNN).
-Apply closedNN.
-Apply iffI.
-Repeat Apply impI.
-Cut (SysPrf
-     (Ensembles.Add (fol.Formula LNN)
-       (Ensembles.Add (fol.Formula LNN) NN
-           (impH
-             (andH
-               (fol.equal LNN (var (S (plus n w))) (natToTerm (Snd a)))
-               (FormulasToFormula (0) w n v))
-             (subAllFormula LNN B
-               [x:nat]
-                Cases x of
-                  0 => (var (0))
-                | (S x') => (var (S (plus x' w)))
-                end)))
-       (fol.equal LNN (var (S (plus n w))) (natToTerm (Snd a))))
-       (impH (FormulasToFormula (0) w n v)
-         (subAllFormula LNN B
-           [x:nat]
-            Cases x of
-              0 => (var (0))
-            | (S x') => (var (S (plus x' w)))
-            end))).
-Generalize (impH
-             (andH
-               (fol.equal LNN (var (S (plus n w))) (natToTerm (Snd a)))
-               (FormulasToFormula (0) w n v))
-             (subAllFormula LNN B
-               [x:nat]
-                Cases x of
-                  0 => (var (0))
-                | (S x') => (var (S (plus x' w)))
-                end)) (impH (FormulasToFormula (0) w n v)
-       (subAllFormula LNN B
-         [x:nat]
-          Cases x of
-            0 => (var (0))
-          | (S x') => (var (S (plus x' w)))
-          end)).
-Cut (lt (plus n w) (S (plus n w))).
-Generalize (S (plus n w)).
-Intros.
-Clear H5 H2 H4 H1 H3 H0 g B v.
-Induction n.
-Simpl.
-Auto.
-Simpl.
-Apply forallI.
-Simpl; Unfold not; Intros.
-Induction H0; Induction H0.
-Induction H1.
-Induction H1.
-Elim closedNN with (plus n (S w)).
-Exists x; Auto.
-Induction H1.
-Simpl in H0.
-Elim (In_list_remove2 ? ? ? ? ? H0).
-Auto.
-Induction H1.
-Induction H0.
-Rewrite <- plus_Snm_nSm in H0.
-Rewrite H0 in H6.
-Elim (lt_n_n ? H6).
-Simpl in H0.
-Elim (closedNatToTerm ? ? H0).
-Apply impE with (fol.equal LNN (var n0) (natToTerm (Snd a))).
-Apply impE with (addForalls (S w) n f).
-Repeat Apply sysWeaken.
-Repeat Apply impI.
-Apply Hrecn.
-EApply lt_trans.
-Apply lt_n_Sn.
-Auto.
-Apply forallSimp with (plus n (S w)).
-Apply Axm; Left; Right; Constructor.
-Apply Axm; Right; Constructor.
-Apply lt_n_Sn.
-Apply impI.
-Apply impE with (andH
-               (fol.equal LNN (var (S (plus n w))) (natToTerm (Snd a)))
-               (FormulasToFormula (0) w n v)).
-Apply Axm; Left; Left; Right; Constructor.
-Apply andI.
-Apply Axm; Left; Right; Constructor.
-Apply Axm; Right; Constructor.
-Apply impI.
-Cut (SysPrf
-     (Ensembles.Add (fol.Formula LNN) NN
-       (impH (fol.equal LNN (var (S (plus n w))) (natToTerm (Snd a)))
-           (impH (FormulasToFormula (0) w n v)
-             (subAllFormula LNN B
-               [x:nat]
-                Cases x of
-                  0 => (var (0))
-                | (S x') => (var (S (plus x' w)))
-                end))))
-       (impH
-         (andH (fol.equal LNN (var (S (plus n w))) (natToTerm (Snd a)))
-           (FormulasToFormula (0) w n v))
-         (subAllFormula LNN B
-           [x:nat]
-            Cases x of
-              0 => (var (0))
-            | (S x') => (var (S (plus x' w)))
-            end))).
-Generalize (impH (FormulasToFormula (0) w n v)
-               (subAllFormula LNN B
-                 [x:nat]
-                  Cases x of
-                    0 => (var (0))
-                  | (S x') => (var (S (plus x' w)))
-                  end))
-(impH
-           (andH
-             (fol.equal LNN (var (S (plus n w))) (natToTerm (Snd a)))
-             (FormulasToFormula (0) w n v))
-           (subAllFormula LNN B
-             [x:nat]
-              Cases x of
-                0 => (var (0))
-              | (S x') => (var (S (plus x' w)))
-              end)).
-Cut (lt (plus n w) (S (plus n w))).
-Generalize (S (plus n w)).
-Intros.
-Clear H5 H2 H4 H1 H3 H0 g B v.
-Induction n.
-Auto.
-Simpl.
-Apply forallI.
-Unfold not; Intros.
-Induction H0; Induction H0.
-Induction H1.
-Elim closedNN with (plus n (S w)).
-Exists x; Auto.
-Induction H1.
-Simpl in H0.
-Induction H0.
-Rewrite <- plus_Snm_nSm in H0.
-Rewrite <- H0 in H6.
-Elim (lt_n_n ? H6).
-NewInduction (in_app_or H0).
-Elim (closedNatToTerm ? ? H1).
-Elim (In_list_remove2 ? ? ? ? ? H1).
-Auto.
-Apply impE with (impH (fol.equal LNN (var n0) (natToTerm (Snd a)))
-         (addForalls (S w) n f)).
-Apply sysWeaken.
-Apply impI.
-Apply Hrecn.
-EApply lt_trans.
-Apply lt_n_Sn.
-Apply H6.
-Apply impI.
-EApply forallSimp.
-Apply impE with (fol.equal LNN (var n0) (natToTerm (Snd a))).
-Apply Axm; Left; Right; Constructor.
-Apply Axm; Right; Constructor.
-Apply lt_n_Sn.
-Apply impI.
-Apply impE with (FormulasToFormula (0) w n v).
-Apply impE with (fol.equal LNN (var (S (plus n w))) (natToTerm (Snd a))).
-Apply Axm; Left; Right; Constructor.
-EApply andE1.
-Apply Axm; Right; Constructor.
-EApply andE2.
-Apply Axm; Right; Constructor.
-Apply iffTrans with (substituteFormula LNN (addForalls (S w) n
-             (impH (FormulasToFormula (0) w n v)
-               (subAllFormula LNN B
-                 [x:nat]
-                  Cases x of
-                    0 => (var (0))
-                  | (S x') => (var (S (plus x' w)))
-                  end))) (plus (S n) w) (natToTerm (Snd a))).
-Rewrite <- plus_Snm_nSm.
-Apply iffI.
-Apply impI.
-Apply impE with (substituteFormula LNN
- (fol.equal LNN (var (S (plus n w))) (natToTerm (Snd a)))
- (S (plus n w)) (natToTerm (Snd a))).
-Rewrite <- (subFormulaImp LNN).
-Apply forallE.
-Apply Axm; Right; Constructor.
-Rewrite subFormulaEqual.
-Rewrite (subTermVar1 LNN).
-Rewrite (subTermNil LNN).
-Apply eqRefl.
-Apply closedNatToTerm.
-Apply impI.
-Apply forallI.
-Unfold not; Intros.
-Induction H6; Induction H6.
-Induction H7.
-Elim closedNN with (plus (S n) w).
-Exists x; Auto.
-Induction H7.
-Simpl in H6.
-NewInduction (freeVarSubFormula3 ? ? ? ? ? H6).
-Elim (In_list_remove2 ? ? ? ? ? H7).
-Auto.
-Elim (closedNatToTerm ? ? H7).
-Apply impI.
-Rewrite <- (subFormulaId LNN (addForalls (S w) n
-       (impH (FormulasToFormula (0) w n v)
-         (subAllFormula LNN B
-           [x:nat]
-            Cases x of
-              0 => (var (0))
-            | (S x') => (var (S (plus x' w)))
-            end))) (S (plus n w))).
-Apply impE with (substituteFormula LNN
-       (addForalls (S w) n
-         (impH (FormulasToFormula (0) w n v)
-           (subAllFormula LNN B
-             [x:nat]
-              Cases x of
-                0 => (var (0))
-              | (S x') => (var (S (plus x' w)))
-              end))) (S (plus n w)) (natToTerm (Snd a))).
-Apply (subWithEquals LNN).
-Apply eqSym.
-Apply Axm; Right; Constructor.
-Rewrite subFormulaId.
-Apply Axm; Left; Right; Constructor.
-Rewrite subAddForallsNice.
-Apply reduceAddForalls.
-Rewrite (subFormulaImp LNN).
-Apply (reduceImp LNN).
-Apply (subFormulaNil LNN).
-Cut (lt (plus n w) (plus (S n) w)).
-Generalize (plus (S n) w).
-Clear H5 H3 g H2.
-Induction v; Unfold not; Intros.
-Simpl in H3.
-Decompose Sum H3.
-Rewrite <- H5 in H2.
-Elim (lt_n_O ? H2).
-Rewrite <- H6 in H2.
-Elim (lt_n_O ? H2).
-Simpl in H3.
-NewInduction (in_app_or H3).
-Simpl in H4.
-NewInduction (freeVarSubFormula3 ? ? ? ? ? H5).
-Elim (le_not_lt n0 O).
-Decompose Record H4.
-Apply H7.
-EApply In_list_remove1.
-Apply H6.
-Apply lt_trans with (plus (S n) w).
-Simpl; Apply lt_O_Sn.
-Auto.
-Induction H6.
-Rewrite <- H6 in H2.
-Elim (lt_n_n ? H2).
-Elim H6.
-Elim Hrecv with n0:=n0.
-Simpl in H4.
-Tauto.
-EApply lt_trans.
-Apply lt_n_Sn.
-Auto.
-Auto.
-Simpl.
-Apply lt_n_Sn.
-EApply iffTrans.
-Apply (subSubAllFormula LNN).
-Apply iffSym.
-EApply iffTrans.
-Apply (subAllSubFormula LNN).
-Replace (subAllFormula LNN B
-         [n1:nat]
-          (substituteTerm LNN
-            Cases n1 of
-              0 => (var (0))
-            | (S x') => (var (S (plus x' w)))
-            end (plus (S n) w) (natToTerm (Snd a))))
-with (subAllFormula LNN B
-         [x:nat]
-          Cases (eq_nat_dec (S n) x) of
-            (left _) => 
-             (subAllTerm LNN (natToTerm (Snd a))
-               [x0:nat]
-                Cases x0 of
-                  0 => (var (0))
-                | (S x') => (var (S (plus x' w)))
-                end)
-          | (right _) => 
-             ([x0:nat]
-               Cases x0 of
-                 0 => (var (0))
-               | (S x') => (var (S (plus x' w)))
-               end x)
-          end).
-Apply iffRefl.
-Apply subAllFormula_ext.
-Intros.
-NewInduction (eq_nat_dec (S n) m).
-Rewrite <- a0.
-Rewrite (subTermVar1 LNN).
-Clear H0.
-NewInduction (Snd a).
-Simpl.
-Reflexivity.
-Simpl.
-Rewrite IHn0.
-Reflexivity.
-NewDestruct m.
-Simpl.
-Reflexivity.
-Rewrite (subTermVar2 LNN).
-Reflexivity.
-Unfold not; Intros; Elim b.
-Apply simpl_plus_l with w.
-Repeat Rewrite (plus_sym w).
-Apply H7.
-Left.
-Rewrite <- (plus_Snm_nSm).
-Apply le_n.
-Intros.
-Elim (closedNatToTerm ? ? H6).
-Apply closedNatToTerm.
-Intros.
-DefinitionTac v' := (vector_rec Formula*(nat->(naryFunc n)) [m:nat][v:(vector ? m)](vector Formula*(naryFunc n) m)
-(Vnil ?)
-[pair:Formula*(nat->(naryFunc n))][m:nat][v:(vector ? m)][rec:(vector Formula*(naryFunc n) m)]
-(Vcons ? ((substituteFormula LNN (Fst pair) (S n) (natToTerm a)),
-          (Snd pair a)) m rec)
-? A).
-Assert (RepresentableHelp n
-                     (evalComposeFunc n m (FormulasToFuncs n m v') g)
-                     (addForalls (S w) m
-                       (impH (FormulasToFormula n w m v')
-                         (subAllFormula LNN B
-                           [x:nat]
-                            Cases x of
-                              0 => (var (0))
-                            | (S x') => (var (S (plus x' w)))
-                            end)))).
-Unfold composePiFormula in Hrecn.
-Simpl in Hrecn.
-Apply Hrecn.
-EApply le_trans.
-Apply le_n_Sn.
-Auto.
-Clear B g H2.
-Induction A;
-Simpl in v';
-Simpl.
-Auto.
-Split.
-Simpl in H0.
-Induction H0.
-Apply H0.
-Apply HrecA.
-Induction H0.
-Auto.
-Simpl in H1.
-Induction H1.
-Auto.
-Simpl in H1.
-Clear H2 H0 g B.
-Induction A.
-Simpl.
-Auto.
-Simpl.
-Split.
-Simpl in H1.
-Induction H1.
-Intros.
-NewInduction (freeVarSubFormula3 ? ? ? ? ? H2).
-Assert (le v (S n)).
-Apply H0.
-EApply In_list_remove1.
-Apply H3.
-NewInduction (le_lt_or_eq ? ? H4).
-Apply lt_n_Sm_le.
-Auto.
-Elim (In_list_remove2 ? ? ? ? ? H3).
-Auto.
-Elim (closedNatToTerm ? ? H3).
-Apply HrecA.
-Induction H1.
-Auto.
-Auto.
-Unfold composePiFormula.
-Clear Hrecn.
-Apply RepresentableAlternate with (addForalls (S w) m
-           (impH (FormulasToFormula n w m v')
-             (subAllFormula LNN B
-               [x:nat]
-                Cases x of
-                  0 => (var (0))
-                | (S x') => (var (S (plus x' w)))
-                end))).
-Rewrite subAddForallsNice.
-Apply reduceAddForalls.
-Rewrite (subFormulaImp LNN).
-Apply (reduceImp LNN).
-Clear H3 H2 H1 H0 g B.
-Induction A.
-Simpl.
-Apply iffSym.
-Apply (subFormulaNil LNN).
-Simpl.
-Unfold not; Intros.
-Decompose Sum H0.
-Discriminate H1.
-Discriminate H2.
-Simpl.
-Rewrite (subFormulaAnd LNN).
-Apply (reduceAnd LNN); [Idtac | Apply HrecA].
-Apply (subFormulaExch LNN).
-Discriminate.
-Apply closedNatToTerm.
-Unfold not; Intros.
-Induction H0.
-Rewrite <- H0 in H.
-Elim (le_not_lt ? ? H).
-Apply le_lt_n_Sm.
-Apply le_plus_r.
-Apply H0.
-Apply iffSym.
-Apply (subFormulaNil LNN).
-Unfold not; Intros.
-Decompose Record (freeVarSubAllFormula1 ? ? ? ? H4).
-NewDestruct x.
-Induction H7.
-Discriminate H5.
-Elim H5.
-Induction H7.
-Rewrite <- H5 in H.
-Elim (le_not_lt ? ? H).
-Apply le_lt_n_Sm.
-Apply le_plus_r.
-Apply H5.
-Right.
-Apply le_lt_n_Sm.
-Auto.
-Intros.
-Elim (closedNatToTerm ? ? H4).
-Apply Representable_ext with (evalComposeFunc n m (FormulasToFuncs n m v') g).
-Clear H3 H2 H1 H0 B.
-Apply extEqualCompose.
-Unfold extEqualVector.
-Clear g.
-Induction A; Simpl.
-Auto.
-Split.
-Apply extEqualRefl.
-Apply HrecA.
-Apply extEqualRefl.
-Apply H3.
-Intros.
-Split.
-Intros.
-Unfold composePiFormula in H4.
-Assert (In v (freeVarFormula LNN
-             (impH (FormulasToFormula n w m A)
-               (subAllFormula LNN B
-                 [x:nat]
-                  Cases x of
-                    0 => (var (0))
-                  | (S x') => (var (plus (S x') w))
-                  end)))).
-EApply freeVarAddForalls1.
-Apply H4.
-Simpl in H5.
-NewInduction (in_app_or H5).
-Assert (le (plus m (S w)) v)\/(lt v (S w)).
-EApply freeVarAddForalls2.
-Apply H4.
-Clear H5 H4 H3 H1 g B.
-Induction A.
-Simpl in H6.
-Decompose Sum H6.
-Rewrite <- H1.
-Apply le_O_n.
-Rewrite <- H3.
-Apply le_O_n.
-Simpl in H6.
-NewInduction (in_app_or H6).
-Simpl in H2.
-Induction H2.
-NewInduction (freeVarSubFormula3 ? ? ? ? ? H1).
-Apply H2.
-EApply In_list_remove1.
-Apply H4.
-Induction H4.
-Rewrite <- H4 in H7.
-Induction H7.
-Rewrite <- plus_Snm_nSm in H5.
-Simpl in H5.
-Elim (le_Sn_n ? H5).
-Elim (lt_not_le ? ? H5).
-Apply le_n_S.
-Apply le_plus_r.
-Elim H4.
-Apply HrecA; Auto.
-Simpl in H2.
-Tauto.
-Induction H7.
-Left.
-Simpl in H3.
-EApply le_trans.
-Apply le_n_Sn.
-Apply H3.
-Auto.
-Decompose Record (freeVarSubAllFormula1 ? ? ? ? H6).
-NewDestruct x.
-Induction H9.
-Rewrite <- H7.
-Apply le_O_n.
-Elim H7.
-Induction H9.
-Rewrite <- H7.
-Induction H3.
-Assert (le (S n0) m).
-Apply H3.
-Auto.
-NewInduction (freeVarAddForalls2 ? ? ? ? H4).
-Rewrite <- H7 in H11.
-Rewrite <- plus_Snm_nSm in H11.
-Simpl in H11.
-Elim (le_not_lt m n0).
-Apply simpl_le_plus_l with w.
-Repeat Rewrite (plus_sym w).
-Apply le_S_n.
-Auto.
-Apply lt_S_n.
-Apply le_lt_n_Sm.
-Auto.
-Rewrite <- H7 in H11.
-Elim (lt_not_le ? ? H11).
-Apply le_n_S.
-Apply le_plus_r.
-Elim H7.
-Apply H; Auto.
-Qed.
-*)
+
+
+
+
+
+
+
+
 
 Remark boundedCheck :
  forall P : nat -> Prop,
@@ -2611,7 +1942,7 @@ Ltac PRsolveFV A B n :=
         assert (In X3 (freeVarFormula LNN X2));
          [ eapply In_list_remove1; apply H
          | assert (X3 <> X1); [ eapply In_list_remove2; apply H | clear H ] ]
-    | H:(In ?X3 (freeVarFormula LNN (fol.andH ?X1 ?X2))) |- _ =>
+    | H:(In ?X3 (freeVarFormula LNN (andH ?X1 ?X2))) |- _ =>
         assert (In X3 (freeVarFormula LNN X1 ++ freeVarFormula LNN X2));
          [ apply H | clear H ]
     | H:(In ?X3 (freeVarFormula LNN (impH ?X1 ?X2))) |- _ =>
