theories/ordinals/MoreAck/LNN_notations.v
@@ -7,47 +7,47 @@ Require Import fol Languages PAtheory LNN.
 Module LNN_notations.
 Declare Scope lnn_scope.
 Delimit Scope lnn_scope with lnn.
-Infix "=" := (fol.equal LNN): lnn_scope.
-Infix "\/" := (fol.orH LNN): lnn_scope.
-Infix "/\" := (fol.andH LNN):lnn_scope.
+Infix "=" := (equal LNN): lnn_scope.
+Infix "\/" := (orH LNN): lnn_scope.
+Infix "/\" := (andH LNN):lnn_scope.
 Infix "->" := (impH LNN): lnn_scope.
-Infix "<->" := (fol.iffH LNN): lnn_scope.
-Notation "~" := (fol.notH LNN): lnn_scope. 
+Infix "<->" := (iffH LNN): lnn_scope.
+Notation "~" := (notH LNN): lnn_scope. 
 
 Set Printing Implicits. 
 Check Zero. 
 Locate Zero. 
-Notation zero := (@fol.apply LNN (Languages.Zero: Functions LNN) (fol.Tnil)).
+Notation zero := (@apply LNN (Languages.Zero: Functions LNN) (fol.Tnil)).
 Check zero.
 
 Notation app1 f arg := 
-  (@fol.apply LNN (f: Functions _) 
-     (fol.Tcons arg (fol.Tnil))).
+  (@apply LNN (f: Functions _) 
+     (Tcons arg (Tnil))).
 
 Notation app2 f arg1 arg2 := 
-  (@fol.apply  LNN (f: Functions _) 
-     (fol.Tcons arg1 (fol.Tcons arg2 (fol.Tnil)))).
+  (@apply  LNN (f: Functions _) 
+     (Tcons arg1 (Tcons arg2 (Tnil)))).
 
-Notation allH := (fol.forallH LNN).
-Notation exH := (fol.existH LNN).
-Notation v_ := (@fol.var LNN).
+Notation allH := (forallH LNN).
+Notation exH := (existH LNN).
+Notation v_ := (@var LNN).
 
 Notation "t1 + t2" := 
-  (fol.apply  LNN Languages.Plus 
-     (fol.Tcons t1 (fol.Tcons t2 (fol.Tnil)))): 
+  (apply  LNN Languages.Plus 
+     (Tcons t1 (Tcons t2 (Tnil)))): 
     lnn_scope.
 
-Notation "t1 * t2" := (fol.apply  LNN Languages.Times 
-     (fol.Tcons  t1 
-        (fol.Tcons  t2 (fol.Tnil)))): lnn_scope.
+Notation "t1 * t2" := (apply  LNN Languages.Times 
+     (Tcons  t1 
+        (Tcons  t2 (Tnil)))): lnn_scope.
 
 Notation S_ t  := (Succ t).
    
 
 Notation "t1 < t2" := 
  (atomic  Languages.LT
-    (fol.Tcons  t1 
-       (fol.Tcons t2 (fol.Tnil)))): lnn_scope.      
+    (Tcons  t1 
+       (Tcons t2 (Tnil)))): lnn_scope.      
  
 End LNN_notations.
 
@@ -58,52 +58,52 @@ Delimit Scope cnn_scope with cnn.
 
 Module CLNN_notations.
 
-Notation "~ A" := (@fol.notH LNN A): cnn_scope.
+Notation "~ A" := (@notH LNN A): cnn_scope.
 
 Notation " A -> B" := (@impH LNN A B) : cnn_scope.
-Notation " A \/ B" := ((@fol.notH LNN  A) -> B)%cnn : cnn_scope.
+Notation " A \/ B" := ((@notH LNN  A) -> B)%cnn : cnn_scope.
 Notation " A /\ B" := 
-     (@fol.notH LNN (@fol.notH LNN  A \/ @fol.notH _ B))%cnn 
+     (@notH LNN (@notH LNN  A \/ @notH _ B))%cnn 
  : cnn_scope.
 
-Notation allH := (@fol.forallH LNN).
+Notation allH := (@forallH LNN).
 
 Notation exH v A := 
-  (@fol.notH _ (@fol.forallH _ v (@fol.notH _ A))).
+  (@notH _ (@forallH _ v (@notH _ A))).
 
 Notation "A <-> B" := (( A -> B) /\ (B -> A))%cnn:  cnn_scope.
 
-Notation "t = u" := (@fol.equal LNN t u): cnn_scope.
+Notation "t = u" := (@equal LNN t u): cnn_scope.
 
-Notation v_ := (@fol.var LNN).
+Notation v_ := (@var LNN).
 
 Notation app1 f arg := 
-  (fol.apply LNN (f: Functions _) 
-     (fol.Tcons  arg (fol.Tnil))).
+  (apply LNN (f: Functions _) 
+     (Tcons  arg (Tnil))).
 
 Notation app2 f arg1 arg2 := 
-  (fol.apply  LNN (f: Functions _) 
-     (fol.Tcons  arg1 (fol.Tcons arg2 (fol.Tnil)))).
+  (apply  LNN (f: Functions _) 
+     (Tcons  arg1 (Tcons arg2 (Tnil)))).
 
-Notation "t1 + t2" := (@fol.apply  LNN Languages.Plus 
-     (fol.Tcons t1 (fol.Tcons  t2 (fol.Tnil)))): cnn_scope.
+Notation "t1 + t2" := (@apply  LNN Languages.Plus 
+     (Tcons t1 (Tcons  t2 (Tnil)))): cnn_scope.
 
-Notation "t1 * t2" := (@fol.apply  LNN Languages.Times 
-     (fol.Tcons  t1 (fol.Tcons  t2 (fol.Tnil)))): cnn_scope.
+Notation "t1 * t2" := (@apply  LNN Languages.Times 
+     (Tcons  t1 (Tcons  t2 (Tnil)))): cnn_scope.
 
 Notation S_ t  := 
-   (@fol.apply  LNN Languages.Succ 
-     (fol.Tcons  t (fol.Tnil))).
+   (@apply  LNN Languages.Succ 
+     (Tcons  t (Tnil))).
 
-About fol.atomic. 
+About atomic. 
 Notation "t1 < t2" := 
- (@fol.atomic LNN Languages.LT
-    (fol.Tcons  t1 
-       (fol.Tcons  t2 (fol.Tnil))))(*only printing*): cnn_scope.      
+ (@atomic LNN Languages.LT
+    (Tcons  t1 
+       (Tcons  t2 (Tnil))))(*only printing*): cnn_scope.      
 
 Print Zero.
 Locate Zero. 
-Definition  zero := (fol.apply (Languages.Zero: Functions LNN) Tnil).
+Definition  zero := (apply (Languages.Zero: Functions LNN) Tnil).
 
  Section Consistance. 
   Goal forall A B, orH  A B = (A \/ B)%cnn. 
